

1. Show $\int_{\mathbb{R}^k} f(x) dx = 1$:

$$f(x) = \frac{1}{\sqrt{(2\pi)^k |\Sigma|}} e^{-\frac{1}{2}(x-\mu)^T \Sigma^{-1}(x-\mu)}$$

1) Let $y = \Sigma^{-\frac{1}{2}}(x-\mu) \Rightarrow x = \mu + \Sigma^{\frac{1}{2}}y$

Jacobian: $\left| \frac{\partial x}{\partial y} \right| = \left| \Sigma^{\frac{1}{2}} \right| = |\Sigma|^{\frac{1}{2}}$

$$\begin{aligned} 2) \int_{\mathbb{R}^k} f(x) dx &= \frac{1}{\sqrt{(2\pi)^k |\Sigma|}} \int_{\mathbb{R}^k} e^{-\frac{1}{2}y^T y} |\Sigma|^{\frac{1}{2}} dy \\ &= \frac{1}{(2\pi)^{\frac{k}{2}}} \int_{\mathbb{R}^k} e^{-\frac{1}{2} \sum_{i=1}^k y_i^2} dy \end{aligned}$$

$$\Rightarrow \int_{\mathbb{R}^k} e^{-\frac{1}{2} \sum_{i=1}^k y_i^2} dy = \prod_{i=1}^k \int_{-\infty}^{\infty} e^{-\frac{y_i^2}{2}} dy_i = (\sqrt{2\pi})^k = (2\pi)^{\frac{k}{2}}$$

$$3) \int_{\mathbb{R}^k} f(x) dx = \frac{(2\pi)^{\frac{k}{2}}}{(2\pi)^{\frac{k}{2}}} = 1$$

2. (a)

$$\frac{\partial}{\partial A} \text{trace}(AB) = B^T$$

<Pf>

$$\text{trace}(AB) = \sum_i (AB)_{ii} = \sum_i \sum_j A_{ij} B_{ji}$$

$$\frac{\partial}{\partial A_{pq}} \text{trace}(AB) = B_{qp}$$

Hence the gradient matrix is B^T . \star

(b)

$$x^T A x = \text{trace}(x \cdot x^T \cdot A)$$

$$x^T A x = \sum_{i,j} x_i A_{ij} x_j$$

$$\begin{aligned} \text{Since } A_{ij} \text{ is constant, } x^T A x &= \sum_{i,j} A_{ij} (x_j x_i) \\ &= \text{trace}(A x x^T) \end{aligned}$$

$$\begin{aligned} \text{By cyclic property of the trace, } x^T A x &= \text{trace}(A x x^T) \\ &= \text{trace}(x x^T A). \quad * \end{aligned}$$

(c)

Let the data x_1, \dots, x_n be i.i.d samples from $\mathcal{N}(\mu, \Sigma)$

$$L(\mu, \Sigma) = \prod_{i=1}^n \frac{1}{(2\pi)^{\frac{n}{2}} |\Sigma|^{\frac{1}{2}}} e^{-\frac{1}{2} (x_i - \mu)^T \Sigma^{-1} (x_i - \mu)}$$

$$l(\mu, \Sigma) = -\frac{n}{2} \log |\Sigma| - \frac{1}{2} \sum_{i=1}^n (x_i - \mu)^T \Sigma^{-1} (x_i - \mu).$$

1)

Define sample scatter matrix:

$$S(\mu) = \sum_{i=1}^n (x_i - \mu) (x_i - \mu)^T$$

$$l(\mu, \Sigma) = -\frac{n}{2} \log |\Sigma| - \frac{1}{2} \log (\Sigma^{-1} S(\mu))$$

$$\therefore dS(\mu) = \sum_{i=1}^n [-d\mu (x_i - \mu)^T - (x_i - \mu) d\mu^T]$$

$$\therefore dl = -\frac{1}{2} \text{trace}(\Sigma^{-1} dS(\mu))$$

$$= -\frac{1}{2} \sum_{i=1}^n \text{trace}(\Sigma^{-1} d\mu (x_i - \mu)^T + \Sigma^{-1} (x_i - \mu) d\mu^T)$$

$$= \sum_{i=1}^n (\Sigma^{-1} (x_i - \mu))^T d\mu$$

$$\frac{\partial l}{\partial \mu} = \Sigma^{-1} \sum_{i=1}^n (x_i - \mu) = 0$$

$$\Rightarrow \hat{\mu} = \frac{1}{n} \sum_{i=1}^n x_i. \quad *$$

2)

With $\mu = \hat{\mu}$

$$l(\Sigma) = -\frac{n}{2} \log |\Sigma| - \frac{1}{2} (\Sigma^{-1} S), \quad S = \sum_{i=1}^n (x_i - \hat{\mu})(x_i - \hat{\mu})^T$$

$$\text{Since } d \log |\Sigma| = \text{trace}(\Sigma^{-1} d\Sigma), \quad d(\Sigma^{-1}) = -\Sigma^{-1} (d\Sigma) \Sigma^{-1}$$

$$dl = -\frac{n}{2} \text{trace}(\Sigma^{-1} d\Sigma) - \frac{1}{2} \text{trace}(d(\Sigma^{-1}) S)$$

$$= -\frac{n}{2} \text{trace}(\Sigma^{-1} d\Sigma) + \frac{1}{2} \text{trace}(\Sigma^{-1} d\Sigma \Sigma^{-1} S)$$

$$= \frac{1}{2} \text{trace}((I - n\Sigma^{-1} + \Sigma^{-1} S \Sigma^{-1}) d\Sigma)$$

For any symmetric $d\Sigma$, set $dl=0$

$$-n\Sigma^{-1} + \Sigma^{-1} S \Sigma^{-1} = 0 \Rightarrow S = n\Sigma$$

$$\text{Thus } \hat{\Sigma} = \frac{1}{n} \sum_{i=1}^n (x_i - \hat{\mu})(x_i - \hat{\mu})^T *$$